Prove axiom6 in hip_graphmark

hip_graphmark_proofs.v
@@ -1,107 +1,122 @@
-Require Import ZArith.
-Require Import hip_graphmark.
+Require Import msl.msl_direct.
+Require Import overlapping.
+Require Import heap_model.
 Require Import graph.
-Require Import List.
+Require Import graph_reachable.
+Require Import spatial_graph.
+Require Import hip_graphmark.
+Require Import utilities.
+Require Import Classical.
+Tactic Notation "LEM" constr(v) := (destruct (classic v); auto).
+
 
 Module GraphMark <: Mgraphmark.
-  Definition formula : Type := Prop.
-  Definition valid (F : formula) : Prop := F.
+  Definition formula : Type := pred world.
+  Definition valid : formula -> Prop := fun f => forall w, f w.
+  Definition node : Type := adr.
+  Definition null_node : node := 0.
+  Definition ptto_node : node -> nat -> node -> node -> formula := trinode.
+  Definition A : Type := @BiMathGraph adr nat 0 natEqDec.
+  Definition graph : node -> A -> formula := spatial_graph.graph.
+  Definition star : formula -> formula -> formula := sepcon.
+  Definition and : formula -> formula -> formula := andp.
+  Definition imp : formula -> formula -> formula := imp.
+  Definition not : formula -> formula := fun f w => ~ f w.
+  Definition eq : node -> node -> formula := fun a b w => a = b.
+  Definition mwand : formula -> formula -> formula := ewand.
+  Definition union : formula -> formula -> formula := ocon.
+  Definition neq : nat -> nat -> formula := fun a b w => ~ a = b.
+  Definition mark : A -> node -> A -> formula :=
+    fun g1 n g2 w => mark adr nat natEqDec (fun d => d = 1) (b_pg_g g1) n (b_pg_g g2).
+  Definition eq_notreach : A -> node -> A -> formula :=
+    fun g1 n g2 w => (unreachable_subgraph (b_pg_g g1) (n :: nil)) -=- (unreachable_subgraph (b_pg_g g2) (n :: nil)).
+  Definition subset_reach : A -> node -> A -> formula :=
+    fun g1 n g2 w => subset (reachable (b_pg_g g1) n) (reachable (b_pg_g g2) n).
+  Definition lookup : A -> node -> nat -> node -> node -> formula :=
+    fun g x d l r w => @node_label _ _ _ (b_pg_g g) x = d /\ @graph.valid _ _ _ (b_pg_g g) x /\
+                       @graph.valid _ _ _ (b_pg_g g) l /\ @graph.valid _ _ _ (b_pg_g g) r /\
+                       (@edge_func _ _ _ (b_pg_g g) x = l :: r :: nil \/ @edge_func _ _ _ (b_pg_g g) x = r :: l :: nil).
+  Definition update : A -> node -> nat -> node -> node -> A -> formula :=
+    fun g1 x d l r g2 w => exists (Hn : x <> 0) (Hi : in_math (bm_ma_g g1) x l r), update_graph g1 x d l r Hi Hn = g2.
 
-  Definition and (F1 F2 : formula) : formula := F1 /\ F2.
-  Definition imp (F1 F2 : formula) : formula := F1 -> F2.
-  Definition not (F : formula) : formula := ~F.
+  Lemma axiom_1 : forall v G1 G2 G G3 x l r, valid (imp (and (lookup G x v l r) (and (mark G r G1) (and (neq v 1) (and (mark G2 l G3) (update G1 x 1 l r G2))))) (and (mark G x G3) (lookup G3 x 1 l r))).
+  Proof. admit. Qed.
   
-  Definition node : Type := Z.
-  Definition null_node : node := 0%Z.
+  Lemma axiom_2 : forall v G1 G2 G G3 x l r, valid (imp (and (lookup G x v l r) (and (mark G l G1) (and (neq v 1) (and (mark G2 r G3) (update G1 x 1 l r G2))))) (and (mark G x G3) (lookup G3 x 1 l r))).
+  Proof. admit. Qed.
   
-  Definition eq (n1 n2 : node) : formula := n1 = n2.
-  Definition neq (z1 z2 : Z) : formula := z1 <> z2.
+  Lemma axiom_3 : forall v G1 G2 G G3 x l r, valid (imp (and (lookup G x v l r) (and (mark G r G1) (and (neq v 1) (and (mark G1 l G2) (update G2 x 1 l r G3))))) (and (mark G x G3) (lookup G3 x 1 l r))).
+  Proof. admit. Qed.
   
-  Instance node_eq_dec : EqDec node.
-  Proof. constructor. unfold node. apply Z_eq_dec. Qed.
+  Lemma axiom_4 : forall v G1 G2 G G3 x l r, valid (imp (and (lookup G x v l r) (and (mark G l G1) (and (neq v 1) (and (mark G1 r G2) (update G2 x 1 l r G3))))) (and (mark G x G3) (lookup G3 x 1 l r))).
+  Proof. admit. Qed.
   
-  (* This needs to be though through some more... *)
-  Definition valid_node (n : node) : Prop := n <> null_node.
-
-  Definition A : Type := @PreGraph node node node_eq_dec valid_node.
+  Lemma axiom_5 : forall v G1 G2 G G3 x l r, valid (imp (and (lookup G x v l r) (and (update G x 1 l r G1) (and (neq v 1) (and (mark G1 r G2) (mark G2 l G3))))) (and (mark G x G3) (lookup G3 x 1 l r))).
+  Proof. admit. Qed.
   
-  Definition lookup (g : A) (n : node) (d : Z) (l r : node) : formula :=
-    @node_label _ _ _ _ g n = d /\
-    @edge_func _ _ _ _ g n = l :: r :: nil.
-  
-  Definition update (g : A) (n : node) (d : Z) (l r : node) (g' : A) : formula :=
-    (forall n', n <> n' -> 
-      (@node_label _ _ _ _ g n' = @node_label _ _ _ _ g' n' /\
-       @edge_func _ _ _ _ g n' = @edge_func _ _ _ _ g' n')) /\
-    @node_label _ _ _ _ g' n = d /\
-    @edge_func _ _ _ _ g' n = l :: r :: nil.
-  
-  Definition marked (g : A) (d : Z) : formula :=
-    d = 1%Z.
-  
-  Lemma lookup_update_mark1: forall g n d l r g',
-    lookup g n d l r ->
-    update g n (1%Z) l r g' ->
-    mark1 _ _ _ _ (marked g') g n g'.
+  Lemma axiom_6 : forall v G1 G2 G G3 x l r, valid (imp (and (lookup G x v l r) (and (update G x 1 l r G1) (and (neq v 1) (and (mark G1 l G2) (mark G2 r G3))))) (and (mark G x G3) (lookup G3 x 1 l r))).
   Proof.
-    intros. split. 
-    red. intros. split. tauto.
-    destruct H as [? ?]. destruct H0 as [? [? ?]].
-    case (t_eq_dec v n). intros. subst n. unfold node in *. rewrite H1,H3. apply eq_as_set_refl.
-    intro. destruct (H0 v). auto.
-    unfold node in *. rewrite H5. apply eq_as_set_refl.
-    split. red. admit. (* need valid proof *)
-    split. red. red. 
-    destruct H0 as [? [? ?]]. apply H1.
-    intros. destruct H0 as [? [? ?]].
-    destruct (H0 n'); auto.
+    intros; intro w; hnf; unfold and; hnf; intros. destruct H as [? [? [? [? ?]]]]. destruct H as [? [? [? [? ?]]]]. hnf in H1.
+    assert (mark1 adr nat natEqDec (fun d : nat => d = 1) (b_pg_g G) x (b_pg_g G1)). destruct H0 as [Hi [Hn ?]].
+    rewrite <- H0. split. intro z. split. destruct (t_eq_dec z x); split; intro. hnf. left; auto. hnf in H8. subst. auto.
+    left; auto. hnf in H8. destruct H8. auto. exfalso; auto. split; intro t; intros. simpl. unfold change_edge_func.
+    destruct (t_eq_dec z x). destruct H7. subst. rewrite H7 in H8. auto. subst. rewrite H7 in H8. apply in_inv in H8.
+    destruct H8. subst. apply in_cons, in_eq. apply in_inv in H; destruct H. subst. apply in_eq. inversion H. auto. simpl in H8.
+    unfold change_edge_func in H8. destruct (t_eq_dec z x). subst. destruct H7. rewrite H. auto. rewrite H. apply in_inv in H8.
+    destruct H8. subst. apply in_cons, in_eq. apply in_inv in H0; destruct H0. subst. apply in_eq. inversion H0. auto.
+    split. auto. split. hnf. simpl. unfold change_node_label. destruct (@t_eq_dec adr natEqDec x x). auto. exfalso; auto.
+    intros. simpl. unfold change_node_label. destruct (t_eq_dec n' x). exfalso; auto. auto. split.
+    apply (mark_mark_mark1 _ _ _ _ (b_pg_g G) (b_pg_g G1) (b_pg_g G2) (b_pg_g G3) x l r). hnf; simpl. rewrite H. auto.
+    split. do 2 (split; auto). destruct H7; rewrite H7. apply in_eq. apply in_cons, in_eq. split. do 2 (split; auto).
+    destruct H7; rewrite H7. apply in_cons, in_eq. apply in_eq. intros. destruct H9 as [?[? ?]].
+    destruct H7; rewrite H7 in H11; apply in_inv in H11; destruct H11. left; auto. apply in_inv in H11. destruct H11.
+    right; auto. inversion H11. right; auto. apply in_inv in H11. destruct H11. left; auto. inversion H11. auto. apply H2.
+    apply H3. destruct H8 as [? [? [? ?]]]. split. hnf in H10. assert (@node_label _ _ _ (b_pg_g G2) x = 1).
+    destruct H2 as [? [? ?]]. specialize (H12 x). specialize (H13 x).
+    LEM ((b_pg_g G1) |= l ~o~> x satisfying (unmarked nat (fun d : nat => d = 1))). specialize (H12 H14). hnf in H12.
+    rewrite H12; auto. specialize (H13 H14). rewrite <- H13. apply H10. destruct H3 as [? [? ?]]. specialize (H13 x).
+    specialize (H14 x). LEM ((b_pg_g G2) |= r ~o~> x satisfying (unmarked nat (fun d : nat => d = 1))). specialize (H13 H15).
+    hnf in H13. auto. specialize (H14 H15). rewrite <- H14. apply H12. destruct H2 as [? _]. destruct H3 as [? _].
+    assert ((b_pg_g G) ~=~ (b_pg_g G2)). apply (si_trans H8 H2). assert ((b_pg_g G) ~=~ (b_pg_g G3)). apply (si_trans H12 H3).
+    hnf in H13. split. destruct (H13 x). rewrite <- H14; auto. split. destruct (H13 l). rewrite <- H14; auto. split.
+    destruct (H13 r). rewrite <- H14; auto. specialize (H13 x). destruct H13.
+    destruct H7; rewrite H7 in H14; destruct H14; hnf in H14, H15;
+    destruct (@only_two_neighbours _ _ _ (bm_bi_g G3) x) as [v1 [v2 ?]]; unfold b_pg_g in *; unfold bm_bi_g in *;
+    rewrite e in *; clear e. assert (In l (l :: r :: nil)). apply in_eq. assert (In r (l :: r :: nil)). apply in_cons, in_eq.
+    generalize (H14 l H16); intro. apply in_inv in H18. destruct H18. subst. left. specialize (H14 r H17).
+    destruct (eq_nat_dec v2 r). subst; auto. assert (In v2 (l :: v2 :: nil)) by apply in_cons, in_eq. specialize (H15 v2 H).
+    clear H16 H17. apply in_inv in H14. apply in_inv in H15. destruct H14, H15; exfalso. rewrite H14 in H15. auto.
+    apply in_inv in H15. destruct H15. auto. inversion H15. apply in_inv in H14. destruct H14. auto. inversion H14.
+    apply in_inv in H14. destruct H14. auto. inversion H14. apply in_inv in H18. destruct H18. right. subst.
+    specialize (H14 r H17). destruct (eq_nat_dec v1 r). subst; auto. assert (In v1 (v1 :: l :: nil)) by apply in_eq.
+    specialize (H15 v1 H). clear H16 H17 H. exfalso. apply in_inv in H14. destruct H14. auto. apply in_inv in H.
+    apply in_inv in H15. destruct H, H15. subst. auto. apply in_inv in H14. destruct H14. auto. inversion H14. inversion H.
+    inversion H. inversion H18. assert (In l (r :: l :: nil)). apply in_cons, in_eq. assert (In r (r :: l :: nil)). apply in_eq.
+    generalize (H14 l H16); intro. apply in_inv in H18. destruct H18. subst. left. specialize (H14 r H17).
+    destruct (eq_nat_dec v2 r). subst; auto. assert (In v2 (l :: v2 :: nil)) by apply in_cons, in_eq. specialize (H15 v2 H).
+    clear H16 H17 H. exfalso. apply in_inv in H15. destruct H15. auto. apply in_inv in H. apply in_inv in H14. destruct H, H14.
+    subst. auto. apply in_inv in H14. destruct H14; [auto | inversion H14]. inversion H. inversion H. apply in_inv in H18.
+    destruct H18. subst. right. specialize (H14 r H17). assert (In v1 (v1 :: l :: nil)). apply in_eq. specialize (H15 v1 H).
+    clear H16 H17 H. destruct (eq_nat_dec v1 r). subst; auto. exfalso. apply in_inv in H14. destruct H14. auto.
+    apply in_inv in H15. destruct H15. auto. apply in_inv in H. apply in_inv in H14. destruct H, H14. subst; auto.
+    inversion H14. inversion H. inversion H14. inversion H18.
   Qed.
- rewrite H1. reflexivity.
-
- trivial.
-
- unfold node_label. hnf. 
- apply sublist_refl.
+  Lemma axiom_7 : forall v G x G1 y v1 l r, valid (imp (and (mark G x G1) (lookup G y v l r)) (and (subset_reach G x G1) (and (eq_notreach G x G1) (lookup G1 y v1 l r)))).
+  Proof. admit. Qed.
+  
+  Lemma axiom_8 : forall l r x G, valid (imp (lookup G x 1 l r) (mark G x G)).
+  Proof. admit. Qed.
+  
+  Lemma axiom_9 : forall G, valid (mark G null_node G).
+  Proof. admit. Qed.
+  
+  Lemma lem_subgraphupdate_l : forall G v G1 x v1 l r, valid (imp (and (star (graph l G1) (mwand (graph l G) (union (ptto_node x v l r) (union (graph l G) (graph r G))))) (and (subset_reach G l G1) (and (eq_notreach G l G1) (and (lookup G x v l r) (lookup G1 x v1 l r))))) (union (ptto_node x v1 l r) (union (graph l G1) (graph r G1)))).
+  Proof. admit. Qed.
+  
+  Lemma lem_subgraphupdate_r : forall G v G1 x v1 l r, valid (imp (and (star (graph r G1) (mwand (graph r G) (union (ptto_node x v l r) (union (graph l G) (graph r G))))) (and (subset_reach G r G1) (and (eq_notreach G r G1) (and (lookup G x v l r) (lookup G1 x v1 l r))))) (union (ptto_node x v1 l r) (union (graph l G1) (graph r G1)))).
+  Proof. admit. Qed.
+  
+  Lemma lem_pttoupdate : forall v G x v1 l r G1, valid (imp (and (star (ptto_node x v1 l r) (mwand (ptto_node x v l r) (union (ptto_node x v l r) (union (graph l G) (graph r G))))) (and (lookup G x v l r) (update G x v1 l r G1))) (union (ptto_node x v1 l r) (union (graph l G1) (graph r G1)))).
+  Proof. admit. Qed.
     
-
- trivial.
-    spec H0 v.
-
-; auto.
-
-    unfold lookup in H. destruct H. rewrite H1.
-    destruct H0. destruct H2.
-
- intro.
-
-apply sublist_refl. intro. 
-    split.  intro. red. red. 
-
-(* SL, empty for now *) 
-  Definition star (F1 F2 : formula) : formula := True.
-  Definition mwand (F1 F2 : formula) : formula := True.
-  Definition union (F1 F2 : formula) : formula := True.
-  Definition ptto_node (n : node) (d : Z) (l r : node) : formula := True.
-  Definition graph (n : node) (g : A) : formula := True.
-(* end SL *)
 End GraphMark.
-
-
-Module Type Mgraphmark.
-  Parameter mark : A -> node -> A -> formula.
-  Parameter eq_notreach : A -> node -> A -> formula.
-  Parameter subset_reach : A -> node -> A -> formula.
-  Axiom axiom_1 : forall v G1 G2 G G3 x l r, valid (imp (and (lookup G x v l r) (and (mark G r G1) (and (neq v 1) (and (mark G2 l G3) (update G1 x 1 l r G2))))) (and (mark G x G3) (lookup G3 x 1 l r))).
-  Axiom axiom_2 : forall v G1 G2 G G3 x l r, valid (imp (and (lookup G x v l r) (and (mark G l G1) (and (neq v 1) (and (mark G2 r G3) (update G1 x 1 l r G2))))) (and (mark G x G3) (lookup G3 x 1 l r))).
-  Axiom axiom_3 : forall v G1 G2 G G3 x l r, valid (imp (and (lookup G x v l r) (and (mark G r G1) (and (neq v 1) (and (mark G1 l G2) (update G2 x 1 l r G3))))) (and (mark G x G3) (lookup G3 x 1 l r))).
-  Axiom axiom_4 : forall v G1 G2 G G3 x l r, valid (imp (and (lookup G x v l r) (and (mark G l G1) (and (neq v 1) (and (mark G1 r G2) (update G2 x 1 l r G3))))) (and (mark G x G3) (lookup G3 x 1 l r))).
-  Axiom axiom_5 : forall v G1 G2 G G3 x l r, valid (imp (and (lookup G x v l r) (and (update G x 1 l r G1) (and (neq v 1) (and (mark G1 r G2) (mark G2 l G3))))) (and (mark G x G3) (lookup G3 x 1 l r))).
-  Axiom axiom_6 : forall v G1 G2 G G3 x l r, valid (imp (and (lookup G x v l r) (and (update G x 1 l r G1) (and (neq v 1) (and (mark G1 l G2) (mark G2 r G3))))) (and (mark G x G3) (lookup G3 x 1 l r))).
-  Axiom axiom_7 : forall v G x G1 y v1 l r, valid (imp (and (mark G x G1) (lookup G y v l r)) (and (subset_reach G x G1) (and (eq_notreach G x G1) (lookup G1 y v1 l r)))).
-  Axiom axiom_8 : forall G x G1, valid (imp (mark G x G1) (and (subset_reach G x G1) (eq_notreach G x G1))).
-  Axiom axiom_9 : forall l r x G, valid (imp (lookup G x 1 l r) (mark G x G)).
-  Axiom axiom_10 : forall G, valid (mark G null_node G).
-  Axiom lem_subgraphupdate_l : forall G v G1 x v1 l r, valid (imp (and (star (graph l G1) (mwand (graph l G) (union (ptto_node x v l r) (union (graph l G) (graph r G))))) (and (subset_reach G l G1) (and (eq_notreach G l G1) (and (lookup G x v l r) (lookup G1 x v1 l r))))) (union (ptto_node x v1 l r) (union (graph l G1) (graph r G1)))).
-  Axiom lem_subgraphupdate_r : forall G v G1 x v1 l r, valid (imp (and (star (graph r G1) (mwand (graph r G) (union (ptto_node x v l r) (union (graph l G) (graph r G))))) (and (subset_reach G r G1) (and (eq_notreach G r G1) (and (lookup G x v l r) (lookup G1 x v1 l r))))) (union (ptto_node x v1 l r) (union (graph l G1) (graph r G1)))).
-  Axiom lem_pttoupdate : forall v1 G1 G x v l r, valid (imp (and (star (ptto_node x v1 l r) (mwand (ptto_node x v l r) (union (ptto_node x v l r) (union (graph l G) (graph r G))))) (lookup G x v l r)) (union (ptto_node x v1 l r) (union (graph l G1) (graph r G1)))).
-End Mgraphmark.
